lib/ExtraLemmas.thy
@@ -1,0 +1,59 @@
+theory ExtraLemmas
+imports AutoCorres
+begin
+
+lemma shiftr1_is_div_2': "shiftr1 (x :: ('a :: len) word) = x div 2"
+apply (simp only: shiftr1_unfold)
+using shiftr1_is_div_2 by auto
+
+lemma shiftr2_is_div_4:
+assumes "2 < len_of TYPE('a)"
+shows "(x :: ('a :: len) word) >> 2 = x div 4"
+proof -
+  from assms have "x >> 2 = x div 2 ^ 2" by (simp add: shiftr_div_2n_w word_size)
+  thus ?thesis by auto
+qed
+
+lemma shiftr3_is_div_8:
+assumes "3 < len_of TYPE('a)"
+shows "(x :: ('a :: len) word) >> 3 = x div 8"
+proof -
+  from assms have "x >> 3 = x div 2 ^ 3" by (simp add: shiftr_div_2n_w word_size)
+  thus ?thesis by auto
+qed
+
+lemma array_addrs_ptr_add[intro]: "0 \<le> i \<Longrightarrow> i < int n \<Longrightarrow> p +\<^sub>p i \<in> set (array_addrs p n)"
+apply (simp add: set_array_addrs)
+apply (rule_tac x="nat i" in exI)
+apply simp
+done
+
+lemma array_addrs_ptr_ex[dest]:
+  "q \<in> set (array_addrs p n)\<Longrightarrow> \<exists>i. q = p +\<^sub>p (int i) \<and> i < n"
+by (simp add: set_array_addrs)
+
+lemma ptr_val_inject: "(p :: 'a ptr) = q \<Longrightarrow> ptr_val p = ptr_val q"
+by auto
+
+lemma ptr_arith_index: "0 \<le> i \<Longrightarrow> 0 \<le> k
+  \<Longrightarrow> nat i * size_of TYPE('a :: wf_type) < 2 ^ len_of TYPE(32)
+  \<Longrightarrow> nat k * size_of TYPE('a :: wf_type) < 2 ^ len_of TYPE(32)
+  \<Longrightarrow> ((p :: 'a ptr) +\<^sub>p i = p +\<^sub>p k) = (i = k)"
+unfolding ptr_add_def
+proof auto
+  fix i k :: int
+  assume size_i: "nat i * size_of TYPE('a) < 4294967296" and "0 \<le> i"
+     and size_k: "nat k * size_of TYPE('a) < 4294967296" and "0 \<le> k"
+     and eq: "of_int i * of_nat (size_of TYPE('a)) = (of_int k * of_nat (size_of TYPE('a)) :: 32 word)"
+  hence "(of_nat (nat i) :: 32 word) * of_nat (size_of TYPE('a))
+    = of_nat (nat k) * of_nat (size_of TYPE('a))" by simp
+  hence "(of_nat (nat i * size_of TYPE('a)) :: 32 word) = of_nat (nat k * size_of TYPE('a))"
+    (is "of_nat ?L = of_nat ?R") by simp
+  moreover have "((of_nat ?L :: 32 word) = of_nat ?R) = (?L = ?R)"
+    using size_i and size_k by (fastforce intro!: WordLemmaBucket.of_nat_inj)
+  ultimately have "?L = ?R" by auto
+  thus "i = k" using not_gr0 sz_nzero
+    by (metis \<open>0 \<le> i\<close> \<open>0 \<le> k\<close> int_nat_eq mult.commute mult_cancel1)
+qed
+
+end
